Repair some more rewrites

Graphiti/Core/Rewrites/BranchMuxToPure.lean
@@ -11,56 +11,51 @@ namespace Graphiti.BranchMuxToPure
 
 open StringModule
 
-variable (T₁ T₂ : Type)
-variable (f g : T₁ → T₂)
-variable (h : Bool × T₁ → T₂)
-variable (S₁ S₂ : String)
+variable (T : Vector Nat 5)
+variable (M : Nat)
 
-def matcher : Pattern String String := fun g => do
+def matcher : Pattern String (String × Nat) 5 := fun g => do
   let (.some list) ← g.modules.foldlM (λ s branch_inst (pmap, branch_typ) => do
        if s.isSome then return s
 
        -- Find the branch
-       unless "branch".isPrefixOf branch_typ do return none
+       unless "branch" == branch_typ.1 do return none
 
        -- Check that the next node is the pure node that also connects to the mux.
        let (.some pure1) := followOutput g branch_inst "out1" | return none
-       unless "pure".isPrefixOf pure1.typ && pure1.incomingPort = "in1" do return none
+       unless "pure" == pure1.typ.1 && pure1.incomingPort = "in1" do return none
 
        let (.some mux) := followOutput g pure1.inst "out1" | return none
-       unless "mux".isPrefixOf mux.typ && mux.incomingPort = "in3" do return none
+       unless "mux" == mux.typ.1 && mux.incomingPort = "in3" do return none
 
        -- Check that the next node is the pure node that also connects to the mux.
        let (.some pure2) := followOutput g branch_inst "out2" | return none
-       unless "pure".isPrefixOf pure2.typ && pure2.incomingPort = "in1" do return none
+       unless "pure" == pure2.typ.1 && pure2.incomingPort = "in1" do return none
 
        let (.some mux') := followOutput g pure2.inst "out1" | return none
-       unless "mux".isPrefixOf mux'.typ && mux'.incomingPort = "in2" && mux.inst = mux'.inst do return none
+       unless "mux" == mux'.typ.1 && mux'.incomingPort = "in2" && mux.inst = mux'.inst do return none
 
-       -- Follow the fork to the mux
+       -- -- Follow the fork to the mux
        let (.some fork) := followInput g branch_inst "in2" | return none
-       unless "fork".isPrefixOf fork.typ && fork.incomingPort == "out1" do return none
+       unless "fork2" == fork.typ.1 && fork.incomingPort == "out1" do return none
 
        let (.some mux'') := followOutput g fork.inst "out2" | return none
        unless mux''.inst = mux.inst && mux''.incomingPort == "in1" do return none
 
-       let (.some t1) := branch_typ.splitOn[1]? | return none
-       let (.some t2) := mux.typ.splitOn[1]? | return none
-
-       return some ([branch_inst, mux.inst, fork.inst, pure1.inst, pure2.inst], [t1, t2])
+       return some ([branch_inst, mux.inst, fork.inst, pure1.inst, pure2.inst], #v[branch_typ.2, mux.typ.2, fork.typ.2, pure1.typ.2, pure2.typ.2])
     ) none | MonadExceptOf.throw RewriteError.done
   return list
 
-def lhs : ExprHigh String String × IdentMap String (TModule1 String) := [graphEnv|
+def lhs : ExprHigh String (String × Nat) := [graph|
     i1 [type = "io"];
     i2 [type = "io"];
     o1 [type = "io"];
 
-    branch [typeImp = $(⟨_, branch T₁⟩), type = $(s!"branch {S₁}")];
-    mux [typeImp = $(⟨_, mux T₂⟩), type = $(s!"mux {S₂}")];
-    fork [typeImp = $(⟨_, fork Bool 2⟩), type = $(s!"fork Bool 2")];
-    pure1 [typeImp = $(⟨_, pure f⟩), type = $(s!"pure {S₁} {S₂}")];
-    pure2 [typeImp = $(⟨_, pure g⟩), type = $(s!"pure {S₁} {S₂}")];
+    branch [type = "branch", arg = $(T[0])];
+    mux [type = "mux", arg = $(T[1])];
+    fork [type = "fork2", arg = $(T[2])];
+    pure1 [type = "pure", arg = $(T[3])];
+    pure2 [type = "pure", arg = $(T[4])];
 
     i1 -> fork [to="in1"];
     i2 -> branch [to="in1"];
@@ -75,19 +70,17 @@ def lhs : ExprHigh String String × IdentMap String (TModule1 String) := [graphE
     mux -> o1 [from="out1"];
   ]
 
-def lhs_extract := (lhs Unit Unit (λ _ => default) (λ _ => default) S₁ S₂).fst.extract ["branch", "mux", "fork", "pure1", "pure2"] |>.get rfl
+def lhs_extract := (lhs T).extract ["branch", "mux", "fork", "pure1", "pure2"] |>.get rfl
+theorem double_check_empty_snd : (lhs_extract T).snd = ExprHigh.mk ∅ ∅ := by rfl
+def lhsLower := lhs_extract T |>.fst.lower.get rfl
 
-theorem double_check_empty_snd : (lhs_extract S₁ S₂).snd = ExprHigh.mk ∅ ∅ := by rfl
-
-def lhsLower := (lhs_extract S₁ S₂).fst.lower.get rfl
-
-def rhs : ExprHigh String String × IdentMap String (TModule1 String) := [graphEnv|
+def rhs : ExprHigh String (String × Nat) := [graph|
     i1 [type = "io"];
     i2 [type = "io"];
     o1 [type = "io"];
 
-    join [typeImp = $(⟨_, join Bool T₁⟩), type = $(s!"join Bool {S₁}")];
-    pure [typeImp = $(⟨_, pure h⟩), type = $(s!"pure (Bool×{S₁}) {S₂}")];
+    join [type = "join", arg = $(M+1)];
+    pure [type = "pure", arg = $(M+2)];
 
     i1 -> join [to="in1"];
     i2 -> join [to="in2"];
@@ -97,26 +90,26 @@ def rhs : ExprHigh String String × IdentMap String (TModule1 String) := [graphE
     join -> pure [from="out1", to="in1"];
   ]
 
-def rhs_extract := (rhs Unit Unit (λ _ => default) S₁ S₂).fst.extract ["join", "pure"] |>.get rfl
+def rhs_extract := (rhs M).extract ["join", "pure"] |>.get rfl
+def rhsLower := (rhs_extract M).fst.lower.get rfl
+def findRhs mod := (rhs_extract 0).fst.modules.find? mod |>.map Prod.fst
 
-def rhsLower := (rhs_extract S₁ S₂).fst.lower.get rfl
-
-def findRhs mod := (rhs_extract "" "").1.modules.find? mod |>.map Prod.fst
-
-def rewrite : Rewrite String String :=
+def rewrite : Rewrite String (String × Nat) :=
   { abstractions := [],
+    params := 5
     pattern := matcher,
-    rewrite := λ | [S₁, S₂] => .some ⟨lhsLower S₁ S₂, rhsLower S₁ S₂⟩ | _ => failure,
+    rewrite := λ l n => ⟨lhsLower l, rhsLower n⟩
     name := "branch-mux-to-pure"
     transformedNodes := [.none, .none, .none, .none, .none]
     addedNodes := [findRhs "join" |>.get rfl, findRhs "pure" |>.get rfl]
+    fresh_types := 2
   }
 
 namespace Test
 
 /-- info: true -/
 #guard_msgs in
-#eval (matcher (lhs_extract "T" "G").1 |>.run' default) == some (["branch", "mux", "fork", "pure1", "pure2"], ["T", "G"])
+#eval matcher (lhs #v[1, 2, 3, 4, 5]) == .ok (["branch", "mux", "fork", "pure1", "pure2"], #v[1, 2, 3, 4, 5])
 
 end Test
 
